io/Free.IO.Sig.fst
@@ -147,13 +147,3 @@ unfold let io_pre (cmd:io_cmds) (arg:io_args cmd) (h:trace) : Type0 =
   | Openfile -> True
   | Read -> is_open arg h
   | Close -> is_open arg h
-
-(** This file is replaced during linking with a file that contains the real
-implementation of the commands. **)
-let io_call (cmd:io_cmds) (arg:io_sig.args cmd) : io (io_sig.res cmd arg) =
-  Call cmd arg Return
-
-(** Since we can lift from io to iio, `iio_call` should be used only for 
-`GetTrace`. **)
-let iio_call (cmd:cmds) (arg:iio_sig.args cmd) : iio (iio_sig.res cmd arg) =
-  Call cmd arg Return
